\documentclass[letterpaper, 12pt]{article}
\usepackage[margin=1in]{geometry}
\usepackage{amsmath}
\usepackage{amssymb}
\usepackage{fancyhdr}
\setlength{\headheight}{15pt}

\pagestyle{fancy}
\fancyhf{}

\rhead{
    Shengdong Li
    Calc 1
}
\rfoot{
    Page \thepage
}

\usepackage{chngcntr}

\counterwithin*{equation}{section}
\counterwithin*{equation}{subsection}

\begin{document}
\title{Initial Post}
\author{by Shengdong Li}
\date{8 May 2020}
\maketitle

\section{$\int_{ }^{ }x^{2}\cos xdx$}
Our goal here is to dissolve the $x^2$. Integration by parts.
\begin{align}
    u  & =x^{2}    \\
    dv & =\cos xdx \\
    du & =2xdx     \\
    v  & =\sin x
\end{align}
Integration by parts again.
\begin{align}
    u  & =2x       \\
    dv & =\sin xdx \\
    du & =2dx      \\
    v  & =-\cos x
\end{align}
\setcounter{equation}{0}
\section{$\int_{ }^{ }\frac{\left(\ln x\right)^{2}}{x}dx$}
U-sub.
\begin{align}
    u  & =\ln x         \\
    du & =\frac{1}{x}dx
\end{align}
\setcounter{equation}{0}
\section{$\int_{ }^{ }\frac{x^{2}}{x+4}dx$}
We want to U-sub to split up the numerator.
\begin{align}
    u     & =x+4                  \\
    x     & =u+4                  \\
    x^{2} & =\left(u+4\right)^{2}
\end{align}
\setcounter{equation}{0}
\section{$\int_{ }^{ }e^{x}\sin xdx$}
The goal here is to get the original integral by doing by parts multiple times.
By parts first.
\begin{align}
    u  & =e^{x}    \\
    dv & =\sin xdx \\
    du & =e^{x}dx  \\
    v  & =-\cos x
\end{align}
By parts again.
\begin{align}
    u  & =e^{x}    \\
    dv & =\cos xdx \\
    du & =e^{x}dx  \\
    v  & =\sin x
\end{align}
\setcounter{equation}{0}
\section{$\int_{ }^{ }x^{3}e^{x^{2}}dx$}
U-sub first.
\begin{align}
    u  & =x^{2} \\
    du & =2x
\end{align}
Then integrate by parts.
\begin{align}
    u  & =u       \\
    dv & =e^{u}du \\
    du & =du      \\
    v  & =e^{u}
\end{align}
\setcounter{equation}{0}
\section{$
      \int_{ }^{ }\cos\left(\sqrt{x}\right)dx
  $}
First u-sub.
\begin{align}
    u                  & =x^{\frac{1}{2}}             \\
    du                 & =\frac{dx}{2x^{\frac{1}{2}}} \\
    2x^{\frac{1}{2}}du & =dx
\end{align}
The components in the $du$ allows us to $u$-sub again. Now we can integrate by parts to dissolve the extra $u$.
\begin{align}
    u  & =u                    \\
    dv & =\cos\left(u\right)du \\
    du & =du                   \\
    v  & =\sin\left(u\right)
\end{align}
\setcounter{equation}{0}
\section{$
      \int_{ }^{ }\frac{\ln x}{x^{5}}dx
  $}
Integrate by parts.
\begin{align}
    u  & =\ln x             \\
    du & =\frac{1}{x}dx     \\
    dv & =x^{-5}dx          \\
    v  & =-\frac{x^{-4}}{4}
\end{align}
\setcounter{equation}{0}
\section{$
      \int_{ }^{ }\frac{xdx}{x^{2}+4x+4}
  $}
Complete the square and then integrate by parts.
\begin{align}
       & \frac{x}{\left(x+2\right)^{2}} \\
    u  & =x+2                           \\
    x  & =u-2                           \\
    du & =dx
\end{align}
\setcounter{equation}{0}
\section{$
      \int_{ }^{ }x\cos\left(x^{2}\right)dx
  $}
Simple u-sub problem.
\begin{align}
    u  & =x^{2} \\
    du & =2xdx
\end{align}
\setcounter{equation}{0}
\section{$
      \int_{ }^{ }\frac{\left(3x^{2}-1\right)dx}{x\left(x^{2}-1\right)}
  $}
Simple u-sub problem.
\begin{align}
    u  & =x^{3}-x    \\
    du & =3x^{2}-1dx
\end{align}
\setcounter{equation}{0}
\section{$
      \int_{ }^{ }\frac{x^{3}}{\sqrt{x^{2}+1}}dx
  $}
U-sub.
\begin{align}
    u     & =x^{2}+1 \\
    x^{2} & =u-1     \\
    du    & =2xdx
\end{align}
\setcounter{equation}{0}
\section{$
    \int_{ }^{ }x^{2}\tan^{-1}xdx
$}
Integrate by parts first to get rid of the $\arctan$
\begin{align}
    u  & =\tan^{-1}x        \\
    du & =\frac{1}{x^{2}+1} \\
    dv & =x^{2}dx           \\
    v  & =\frac{x^{3}}{3}
\end{align}
Then u-sub
\begin{align}
    u     & =x^{2}+1 \\
    x^{2} & =u-1     \\
    du    & =2xdx
\end{align}
\end{document}