\documentclass[letterpaper, 12pt]{article}
\usepackage[margin=1in]{geometry}
\usepackage{amsmath}
\usepackage{amssymb}
\usepackage{fancyhdr}
\setlength{\headheight}{15pt}

\pagestyle{fancy}
\fancyhf{}

\rhead{
    Shengdong Li
    Calc 1
}
\rfoot{
    Page \thepage
}

\usepackage{indentfirst}

\begin{document}
\title{Response to Nancy Bai}
\author{by Shengdong Li}
\date{10 May 2020}
\maketitle

\section{Intro}
Hey Nancy! I just wanted to say that while it probably wasn't the best solution for the for $\int_{ }^{ }x^{3}e^{x^{2}}dx$, your method of manipulation of $u$-sub and then $v$-sub for this problem was absolutely ingenious, and I wouldn't have seen it in a million years if you hadn't shown me your stub values. \par
That being said, it took me a rather long time to work through this problem using your solution, so I wanted to provide a more detailed and in-depth walkthrough of how to go through this problem using $u$-sub and then $v$-sub
\section{Solution}
\noindent Let's restate the problem first
\begin{align}
&\int_{ }^{ }x^{3}e^{x^{2}}dx
\intertext{Now use the incredible $u=x^3$}
u&=x^3
\intertext{Now instead of plugging in this $u$ value immediately, let's first take the derivative of both sides}
du&=3x^{2}dx\\
\frac{du}{3x^{2}}&=dx
\intertext{Then plug that in, which results in}
&=\frac{1}{3}\int_{ }^{ }xe^{x^{2}}du
\intertext{Now we manipulate $u$ to account for these specific $x$ values...}
u^{\frac{2}{3}}&=x^{2}\\
u^{\frac{1}{3}}&=x
\intertext{And finally complete the $u$-sub}
&=\frac{1}{3}\int_{ }^{ }u^{\frac{1}{3}}e^{u^{\frac{2}{3}}}du
\intertext{Now onto the $v$-sub}
v&=u^{\frac{2}{3}}\\
dv&=\frac{2u^{-\frac{1}{3}}}{3}du\\
dv&=\frac{2}{3u^{\frac{1}{3}}}du\\
\frac{3}{2}u^{\frac{1}{3}}dv&=du
\intertext{And plugging in what we have far reveals another possible $v$-sub from the components of the $dv$}
&=\frac{1}{3}\cdot\frac{3}{2}\int_{ }^{ }u^{\frac{2}{3}}e^{v}dv
\intertext{Which, after distributing and simplifying factors, gives us a really simple expression}
&=\frac{1}{2}\int_{ }^{ }ve^{v}dv
\intertext{Now we can integrate by parts, and resub to put in terms of $x$ again}
u&=v\\
dv&=e^{v}dv\\
du&=dv\\
v&=e^{v}\\
&=\frac{1}{2}\left(ve^{v}-\int_{ }^{ }e^{v}dv\right)\\
&=\frac{1}{2}\left(ve^{v}-e^{v}\right)\\
&=\frac{1}{2}\left(u^{\frac{2}{3}}e^{u^{\frac{2}{3}}}-e^{u^{\frac{2}{3}}}\right)\\
&=\frac{1}{2}\left(\left(x^{3}\right)^{\frac{2}{3}}e^{\left(x^{3}\right)^{\frac{2}{3}}}-e^{\left(x^{3}\right)^{\frac{2}{3}}}\right)\\
&=\boxed{\frac{1}{2}\left(x^{2}e^{x^{2}}-e^{x^{2}}\right)+C}
\end{align}
\section{Conclusion}
I got stuck for multiple minutes at multiple sections of this problem using $u$-sub and $v$-sub, and again, would have never thought of this solution in a million years. Great job of thinking up this solution Nancy!!
\end{document}