\documentclass[letterpaper, 12pt]{article}
\usepackage[margin=1in]{geometry}
\usepackage{amsmath}
\usepackage{amssymb}
\usepackage{fancyhdr}

\pagestyle{fancy}
\fancyhf{}
\rhead{
    Shendong Li
    Calc 1
}
\rfoot{
    Page \thepage
}

\begin{document}
\title{(Verification) Response to Andrew Fleischer}
\author{by Shengdong Li}
\date{2 May 2020}
\maketitle
\section{Intro}
Hello Andrew! I'll try to verify your problem. 
\section{Solution}
\begin{align}
    \intertext{Because the funtion is defining velocity, to find total distance travelled from $0$ to $t$, we just need to integrate the function from $0$ to $t$, which looks something like this:}
    &\int_{0}^{t}t^{2}e^{-4t}dt
    \intertext{From here we need to integrate by parts. Recalling the integration by parts formula here...}
    \int_{ }^{ }f\left(x\right)g'\left(x\right)dx&=f\left(x\right)g\left(x\right)-\int_{ }^{ }f'\left(x\right)g\left(x\right)dx
    \intertext{Define the $u$ and $dv$ functions for the integral at hand, then find the $du$ and $v$ functions}
    u&=t^{2}\\
    dv&=e^{-4t}\ dt\\
    du&=2t\ dt\\
    v&=-\frac{e^{-4t}}{4}
    \intertext{Plugin to the integration by parts formula}
    &=-\frac{t^{2}e^{-4t}}{4}\Big|_{0}^{t}-\int_{0}^{t}\ -\frac{2te^{-4t}}{4}dt
    \intertext{The definite integral cancels here when $t=0$}
    &=-\frac{t^{2}e^{-4t}}{4}-\int_{0}^{t}\ -\frac{2te^{-4t}}{4}dt
    \intertext{Factor out the inside of the integral}
    &=-\frac{t^{2}e^{-4t}}{4}+\frac{1}{2}\int_{0}^{t}\ te^{-4t}dt
    \intertext{Define the $u$ and $dv$ functions for the new integral at hand, then find the $du$ and $v$ functions}
    u&=t\\
    dv&=e^{-4t}\ dt\\
    du&=dt\\
    v&=-\frac{e^{-4t}}{4}
    \intertext{Plugin to the integration by parts equation}
    &=-\frac{t^{2}e^{-4t}}{4}+\frac{1}{2}\left(-\frac{te^{-4t}}{4}\Big|_{0}^{t}-\int_{0}^{t}\ -\frac{e^{-4t}}{4}dt\right)
    \intertext{The definite integrals cancel here again when $t=0$}
    &=-\frac{t^{2}e^{-4t}}{4}+\frac{1}{2}\left(-\frac{te^{-4t}}{4}-\int_{0}^{t}\ -\frac{e^{-4t}}{4}dt\right)
    \intertext{Factor out the inside of the integral}
    &=-\frac{t^{2}e^{-4t}}{4}+\frac{1}{2}\left(-\frac{te^{-4t}}{4}+\frac{1}{4}\int_{0}^{t}\ e^{-4t}dt\right)
    \intertext{Integrate the inside of the expression}
    &=-\frac{t^{2}e^{-4t}}{4}+\frac{1}{2}\left(-\frac{te^{-4t}}{4}+\frac{1}{4}\left(-\frac{e^{-4t}}{4}\Big|_{0}^{t}\right)\right)
    \intertext{The definite integral doesn't cancel this time}
    &=-\frac{t^{2}e^{-4t}}{4}+\frac{1}{2}\left(-\frac{te^{-4t}}{4}+\frac{1}{4}\left(-\frac{e^{-4t}}{4}-\left(-\frac{1}{4}\right)\right)\right)
    \intertext{Now we can just simplify}
    &=-\frac{t^{2}e^{-4t}}{4}+\frac{1}{2}\left(-\frac{te^{-4t}}{4}+\frac{1}{4}\left(-\frac{e^{-4t}}{4}+\frac{1}{4}\right)\right)\\
    &=-\frac{t^{2}e^{-4t}}{4}+\frac{1}{2}\left(-\frac{te^{-4t}}{4}-\frac{e^{-4t}}{16}+\frac{1}{16}\right)\\
    &=-\frac{t^{2}e^{-4t}}{4}-\frac{te^{-4t}}{8}-\frac{e^{-4t}}{32}+\frac{1}{32}
    \intertext{\textbf{It's very important here to note that the $\frac{1}{32}$ just gets sucked up by the $+C$, and you're left with just}}
    &=-\frac{t^{2}e^{-4t}}{4}-\frac{te^{-4t}}{8}-\frac{e^{-4t}}{32}+c
    \intertext{I've definitely gotten a problem wrong on not just the \textit{practice test} by not removing the consant value... You could also factor, which matches Yuangchang's comment above...}
    &=\boxed{\frac{-e^{-4t}}{32}\left(8t^{2}+4t+1\right)+c}
\end{align}
\section{Conclusion}
I hope that my comment helped!
\bigskip
\par
Cheers, 
\par
Andy Li
\end{document}